Split saved_interp_dep out of hoInterps_experiments.v

theories/hoInterps_experiments.v
@@ -1,21 +1,17 @@
 From iris.proofmode Require Import tactics.
 From iris.base_logic Require Import lib.saved_prop.
 From D Require Import prelude iris_prelude saved_interp_n.
-Import uPred.
-
-Unset Program Cases.
-(* Repeat temporarily-disabled Iris notations. *)
-Notation "{ x  &  P }" := (sigTOF (λ x, P%OF)) : oFunctor_scope.
-Notation "{ x : A &  P }" := (@sigTOF A%type (λ x, P%OF)) : oFunctor_scope.
+From D Require Import saved_interp_dep.
+Import uPred EqNotations.
 
 Module try1.
 Section saved_pred3_use.
   Context {vl : Type} {Σ : gFunctors}.
 
-  Notation envD Σ := ((var → vl) -d> vl -d> iProp Σ).
-  Notation hoEnvD Σ := (list vl -d> envD Σ).
+  Notation _envD Σ := ((var → vl) -d> vl -d> iProp Σ).
+  Notation hoEnvD Σ := (list vl -d> _envD Σ).
   Implicit Types (Φ : hoEnvD Σ) (n : nat).
-  Definition eFalse : envD Σ := λ ρ v, False%I.
+  Definition eFalse : _envD Σ := λ ρ v, False%I.
 
   (* We can track function arity by just storing a number,
      but that's a bit cumbersome. *)
@@ -25,7 +21,7 @@ Section saved_pred3_use.
     | 0 => (0, λ _, eFalse)
     | S n => (n, λ args, Φ (a :: args))
     end%I.
-  Definition close : hoEnvND Σ → envD Σ := λ '(n, Φ), Φ [].
+  Definition close : hoEnvND Σ → _envD Σ := λ '(n, Φ), Φ [].
   Definition lambda n (Φ : vl → hoEnvD Σ) : hoEnvND Σ :=
     (n + 1, λ args,
       match args with
@@ -36,8 +32,6 @@ End saved_pred3_use.
 End try1.
 
 Module try2.
-
-Definition vec n vl := fin n → vl.
 Section vec.
   Context {vl : Type}.
   (* vector operations, on a functional representation of vectors. *)
@@ -52,61 +46,42 @@ Section vec.
   Definition vhead {n} (args: vec (S n) vl) : vl := args Fin.F1.
   Definition vtail {n} (args: vec (S n) vl) : fin n → vl :=
     λ i, args (Fin.FS i).
-End vec.
 
-(* To prove saved_pred3_own_contractive, below, we need to hide n under ▶. *)
-Definition mFun vl : oFunctor := { n & vec n vl -d> (var → vl) -d> vl -d> ▶ ∙ }.
-Notation savedPred3G Σ vl := (savedAnythingG Σ (mFun vl)).
-Notation savedPred3Σ vl := (savedAnythingΣ (mFun vl)).
-From D Require Import asubst_intf dlang olty.
-
-Module Foo (values: Values) (sorts: SortsIntf values).
-  Module M := (OLty values sorts).
-  Module N := LiftWp values sorts.
-  Import M N values.
-  Notation envD Σ := ((var → vl) -d> vl -d> iProp Σ).
-  Notation hoEnvND n Σ := (vec n vl -d> envD Σ).
-
-Section saved_pred3.
-  Import EqNotations.
-
-  (* For Iris. *)
-
-  Global Instance projT1_ne {A P}: NonExpansive (projT1: @sigTO A P → leibnizO A).
-  Proof. solve_proper. Qed.
-
-  Lemma projT2_ne {A P}: ∀ n (x1 x2 : @sigTO A P) (Heq : x1 ≡{n}≡ x2),
-    rew (sigT_dist_proj1 n Heq) in projT2 x1 ≡{n}≡ projT2 x2.
-  Proof. by destruct Heq. Qed.
-
-  Context `{!savedPred3G Σ vl}.
-
-  Definition hoEnvD_P Σ := (λ n, hoEnvND n Σ).
-  Definition hoEnvDO Σ : ofeT := sigTO (hoEnvD_P Σ).
-
-  Definition packedFun : ofeT := mFun vl (iProp Σ) uPred_cofe.
-  Definition packedFun_eq : packedFun =
-    sigTO (λ n, vec n vl -d> (var → vl) -d> vl -d> laterO (iProp Σ)) := reflexivity _.
-
-  Definition packedFun_arity : packedFun -n> natO := λne x, projT1 x.
-
-  Implicit Types (Ψ : packedFun).
-
-  (* Manipulate *)
+  (* Manipulation of higher-order semantic types. *)
   Definition close {A} (Φ : vec 0 vl -d> A): A := Φ emptyArgs.
 
   Definition beta {n A} (Φ : vec (S n) vl -d> A) v : vec n vl -d> A :=
     λ args, Φ (vcons v args).
 
-  Definition lambda {n A} (Φ : vl → vec n vl -d> A) : vec (S n) vl -d> A :=
+  Definition lambda {n A} (Φ : vl → vec n vl -d> A) :
+    vec (S n) vl -d> A :=
     λ args, Φ (vhead args) (vtail args).
+End vec.
 
-  (* Right definition? *)
-  Definition subtype {n} (φ1 φ2 : hoEnvND n Σ) ρ : iProp Σ :=
-    (∀ (args : vec n vl) v, φ1 args ρ v -∗ φ2 args ρ v)%I.
+From D Require Import asubst_intf dlang olty.
+
+Module HoSemTypes (values: Values) (sorts: SortsIntf values).
+
+(* Module M := (OLty values sorts). Import M. *)
+Import values sorts.
+
+Notation _envD Σ := ((var → vl) -d> vl -d> iProp Σ).
+Notation hoEnvND n Σ := (vec n vl -d> _envD Σ).
+Definition hoD n Σ := vec n vl -d> vl -d> iProp Σ.
+
+Section saved_ho_sem_type_extra.
+  Context `{!savedHoSemTypeG vl Σ}.
+
+  Implicit Types (Ψ : packedFun vl Σ).
+
+  Definition subtype {n} i j (φ1 φ2 : hoD n Σ) : iProp Σ :=
+    (□∀ (args : vec n vl) v, ⌜ nclosed_vl v 0 ⌝ →
+      ▷^i φ1 args v -∗ ▷^j φ2 args v)%I.
+  Definition semEquiv {n} i j (φ1 φ2 : hoD n Σ) : iProp Σ :=
+    (□∀ (args : vec n vl) v, ⌜ nclosed_vl v 0 ⌝ → ▷^i φ1 args v ∗-∗ ▷^j φ2 args v)%I.
 
   Fixpoint subtype_w_expKind ρ n :
-      ∀ (φ1 φ2 : hoEnvND n Σ) (argTs : vec n (envD Σ)), iProp Σ :=
+      ∀ (φ1 φ2 : hoEnvND n Σ) (argTs : vec n (_envD Σ)), iProp Σ :=
     match n with
     | 0 =>   λ φ1 φ2 argTs,
         ∀ v, close φ1 ρ v -∗ close φ2 ρ v
@@ -115,106 +90,40 @@ Section saved_pred3.
           subtype_w_expKind ρ n (beta φ1 v) (beta φ2 v) (vtail argTs)
     end%I.
 
-  Definition cpack n : hoEnvND n Σ → packedFun :=
-    λ Φf, existT n (λ args ρ v, Next (Φf args ρ v)).
-
-  Global Instance cpack_contractive: Contractive (cpack n).
-  Proof.
-    rewrite /cpack => ?????.
-    apply (existT_ne _ eq_refl).
-    solve_contractive_ho.
-  Qed.
-  Program Definition pack : hoEnvDO Σ -n> packedFun :=
-    λne '(existT n Φ), cpack n Φ.
-  Next Obligation.
-    move => ?[??][??][/= Heq ?]. destruct Heq. by f_equiv.
-  Qed.
-
-  Definition saved_pred3_own γ i (Φ : hoEnvND i Σ) : iProp Σ :=
-    saved_anything_own (F := mFun vl) γ (pack (existT i Φ)).
-
-  Notation "γ ⤇[ i  ] φ" := (saved_pred3_own γ i φ) (at level 20).
-
-  Instance saved_pred3_own_contractive γ i : Contractive (saved_pred3_own γ i).
-  Proof.
-    rewrite /saved_pred3_own => n f g /= Heq. f_equiv.
-    apply (existT_ne _ eq_refl) => ??? /=.
-    solve_contractive_ho.
-  Qed.
-
-  Lemma saved_pred3_alloc i φ : (|==> ∃ γ, γ ⤇[ i ] φ)%I.
-  Proof. apply saved_anything_alloc. Qed.
-
-  Lemma same_arity_1 {Φ Ψ : packedFun} {n} :
+  Lemma packedFun_arity_ne {Φ Ψ : packedFun vl Σ} {n} :
     Φ ≡{n}≡ Ψ → packedFun_arity Φ = packedFun_arity Ψ.
-  Proof. destruct Φ, Ψ. by case. Qed.
+  Proof. apply packedFun_arity. Qed.
 
-  Lemma same_arity Ψ1 Ψ2 : Ψ1 ≡ Ψ2 -∗
-    ⌜ packedFun_arity Ψ1 = packedFun_arity Ψ2 ⌝: iProp Σ.
-  Proof. rewrite /= sigT_equivI. by iDestruct 1 as (Heq) "_". Qed.
+  Program Definition unNext: laterO (iProp Σ) -n> iProp Σ :=
+    λne φ, (▷ later_car φ)%I.
+  Next Obligation. solve_contractive. Qed.
 
-  Lemma saved_pred3_agree_arity γ {i j Φ1 Φ2}:
-    γ ⤇[ i ] Φ1 -∗ γ ⤇[ j ] Φ2 -∗ ⌜ i = j ⌝.
+  Definition unpack : ∀ Ψ, hoEnvND (packedFun_arity Ψ) Σ :=
+    λ Ψ args ρ v, unNext (projT2 Ψ args ρ v).
+
+  Lemma unpack_ne {n Ψ1 Ψ2} (Heq : Ψ1 ≡{n}≡ Ψ2):
+    rew [hoEnvD_P vl Σ] (packedFun_arity_ne Heq) in unpack Ψ1 ≡{n}≡ unpack Ψ2.
   Proof.
-    iIntros "HΦ1 HΦ2 /=".
-    iDestruct (saved_anything_agree with "HΦ1 HΦ2") as "Heq".
-    by rewrite same_arity.
+    move: Ψ1 Ψ2 Heq (packedFun_arity_ne Heq) => [/= n1 Φ1] [/= n2 Φ2] [/= Heq1 Heq] HeqN.
+    move: Heq; rewrite (proof_irrel HeqN Heq1) /unpack /=.
+    destruct Heq1 => /= H ???. f_contractive. exact: H.
   Qed.
 
-  Lemma saved_pred3_agree γ i (Φ1 Φ2 : hoEnvND i Σ) a b c:
-    γ ⤇[ i ] Φ1 -∗ γ ⤇[ i ] Φ2 -∗ ▷ (Φ1 a b c ≡ Φ2 a b c).
-  Proof.
-    iIntros "HΦ1 HΦ2 /=".
-    iDestruct (saved_anything_agree with "HΦ1 HΦ2") as "Heq".
-    rewrite /= sigT_equivI. iDestruct "Heq" as (Heq) "Heq".
-    rewrite (proof_irrel Heq eq_refl) /=.
-    repeat setoid_rewrite bi.discrete_fun_equivI; iNext.
-    iApply "Heq".
-  Qed.
+  Lemma unpack_ne_eta n Ψ1 Ψ2 (Heq : Ψ1 ≡{n}≡ Ψ2) a b c:
+    (rew [hoEnvD_P vl Σ] (packedFun_arity_ne Heq) in unpack Ψ1) a b c ≡{n}≡
+    unpack Ψ2 a b c.
+  Proof. exact: unpack_ne. Qed.
+End saved_ho_sem_type_extra.
+End HoSemTypes.
 
-  Lemma saved_pred3_agree_dep γ {i j Φ1 Φ2} a b c:
-    γ ⤇[ i ] Φ1 -∗ γ ⤇[ j ] Φ2 -∗ ∃ eq : i = j,
-    ▷ ((rew [hoEnvD_P Σ] eq in Φ1) a b c ≡ Φ2 a b c).
-  Proof.
-    iIntros "HΦ1 HΦ2 /=".
-    iDestruct (saved_pred3_agree_arity with "HΦ1 HΦ2") as %->.
-    iExists eq_refl; cbn.
-    iApply (saved_pred3_agree with "HΦ1 HΦ2").
-  Qed.
+Notation "s ↝[ n ] φ" := (∃ γ, (s ↦ γ) ∗ (γ ⤇[ n ] φ))%I  (at level 20) : bi_scope.
 
-  Definition unpack :
-    ∀ Ψ, hoEnvND (packedFun_arity Ψ) Σ :=
-    λ '(existT n Φ), (λ args ρ v,
-      let '(Next f) := (Φ args ρ v) in f)%I.
-
-  Lemma pred_impl (Φ Ψ : packedFun) n (Heq: Φ ≡{n}≡ Ψ)
-    (a : vec (packedFun_arity Φ) vl) b c:
-    Next (unpack Φ a b c) ≡{n}≡ Next (unpack Ψ (rew [λ n, vec n vl] (same_arity_1 Heq) in a) b c).
-  Proof.
-    move: (same_arity_1 Heq) => HeqN. destruct Φ, Ψ; simpl in *.
-    case: Heq => /= Heq1.
-    have {HeqN} ->: HeqN = Heq1. exact: proof_irrel.
-    destruct Heq1; cbn => H. exact: H.
-  Qed.
-  Notation "s ↝[ i ] φ" := (∃ γ, (s ↦ γ) ∗ (γ ⤇[ i ] φ))%I  (at level 20) : bi_scope.
-
-End saved_pred3.
-
-Opaque saved_pred3_own.
-
-Notation "γ ⤇[ i ] φ" := (saved_pred3_own γ i φ) (at level 20).
-Notation "s ↝[ i ] φ" := (∃ γ, (s ↦ γ) ∗ (γ ⤇[ i ] φ))%I  (at level 20) : bi_scope.
-
-End Foo.
-From D.Dot Require Import syn unary_lr.
-Include Foo syn syn.
+From D.Dot Require Import syn operational.
+Include HoSemTypes syn syn.
 
 Section bar.
-  Context `{!savedPred3G Σ vl} `{!N.dlangG Σ}.
-  (* Implicit Types (interp : envD Σ) (φ : D). *)
-About saved_pred3_own.
-
-  Definition hoD n Σ := vec n vl -d> vl -d> iProp Σ.
+  Context `{!savedHoSemTypeG vl Σ} `{!dlangG Σ}.
+  (* Implicit Types (interp : _envD Σ) (φ : D). *)
 
   Definition idm_proj_semtype (d : dm) n (φ : hoD n Σ) : iProp Σ :=
     (∃ s σ interp,
@@ -225,18 +134,15 @@ About saved_pred3_own.
   Notation "d ↗[ n ] φ" := (idm_proj_semtype d n φ) (at level 20).
 
   Notation envPred s := (vls -d> s -d> iProp Σ).
-  Definition subtype' {n} i j (φ1 φ2 : hoD n Σ) : iProp Σ :=
-    (□∀ (args : vec n vl) v, ⌜ nclosed_vl v 0 ⌝ → ▷^i φ1 args v -∗ ▷^j φ2 args v)%I.
-  Definition semEquiv {n} i j (φ1 φ2 : hoD n Σ) : iProp Σ :=
-    (□∀ (args : vec n vl) v, ⌜ nclosed_vl v 0 ⌝ → ▷^i φ1 args v ∗-∗ ▷^j φ2 args v)%I.
+
 
   Definition kind n Σ := hoD n Σ → iProp Σ.
 
   (* The point of Sandro's kind syntax is to use this only at kind 0. *)
   (* Definition ktmem {n} (φ1 φ2 : hoD n Σ) φ :=
-    (subtype' n 1 1 φ1 φ ∗ subtype' n 1 1 φ φ)%I. *)
+    (subtype n 1 1 φ1 φ ∗ subtype n 1 1 φ φ)%I. *)
   Definition ktmem (φ1 φ2 : hoD 0 Σ) φ :=
-    (subtype' 1 1 φ1 φ ∗ subtype' 1 1 φ φ)%I.
+    (subtype 1 1 φ1 φ ∗ subtype 1 1 φ φ)%I.
 
   Definition kpi {n} (K : kind n Σ) (φ₁ : hoD 0 Σ) : kind (S n) Σ :=
     λ φ, (□∀ arg, close φ₁ arg → K (beta φ arg))%I.
@@ -254,7 +160,7 @@ About saved_pred3_own.
     on arbitrary arguments — they might, at best, become False on bad
     ones. *)
   Definition lam_subtype {n} (argT : hoD 0 Σ) (φ1 φ2 : hoD (S n) Σ) :=
-    (□∀ arg, □close argT arg -∗ subtype' 0 0 (beta φ1 arg) (beta φ2 arg))%I.
+    (□∀ arg, □close argT arg -∗ subtype 0 0 (beta φ1 arg) (beta φ2 arg))%I.
 
   Definition lam_semEquiv {n} (argT : hoD 0 Σ) (φ1 φ2 : hoD (S n) Σ) :=
     (□∀ arg, □close argT arg -∗ semEquiv 0 0 (beta φ1 arg) (beta φ2 arg))%I.
@@ -262,7 +168,7 @@ About saved_pred3_own.
   (* Here, we inherit eta from the metalanguage, in both directions. *)
   Lemma eta1 {n} argT (φ : hoD (S n) Σ): lam_subtype argT φ (λ v, φ v).
   Proof.
-    rewrite /lam_subtype /subtype' /beta /=.
+    rewrite /lam_subtype /subtype /beta /=.
     iIntros "!>" (arg) "#Harg !>"; iIntros (args v Hcl) "? //".
   Qed.
 
@@ -274,3 +180,4 @@ About saved_pred3_own.
   Qed.
 End bar.
 
+Notation "d ↗[ n ] φ" := (idm_proj_semtype d n φ) (at level 20).
