theories/saved_interp_dep.v
@@ -1,0 +1,117 @@
+From iris.proofmode Require Import tactics.
+From iris.base_logic Require Import lib.saved_prop.
+From D Require Import prelude iris_prelude.
+
+Import uPred EqNotations.
+Unset Program Cases.
+
+(* Repeat temporarily-disabled Iris notations. *)
+Notation "{ x  &  P }" := (sigTOF (λ x, P%OF)) : oFunctor_scope.
+Notation "{ x : A &  P }" := (@sigTOF A%type (λ x, P%OF)) : oFunctor_scope.
+Definition vec n vl := fin n → vl.
+
+Notation _envD vl Σ := ((var → vl) -d> vl -d> iProp Σ).
+Notation hoEnvND n vl Σ := (vec n vl -d> _envD vl Σ).
+
+Definition hoEnvD_P vl Σ := (λ n, hoEnvND n vl Σ).
+Definition hoEnvDO vl Σ : ofeT := sigTO (hoEnvD_P vl Σ).
+
+Definition hoEnvDOF vl : oFunctor := { n & vec n vl -d> (var → vl) -d> vl -d> ▶ ∙ }.
+
+Notation savedHoSemTypeG vl Σ := (savedAnythingG Σ (hoEnvDOF vl)).
+Notation savedHoSemTypeΣ vl := (savedAnythingΣ (hoEnvDOF vl)).
+
+Definition packedFun vl Σ : ofeT := hoEnvDOF vl (iProp Σ) _.
+
+(* For Iris. *)
+Global Instance projT1_ne {A P}: NonExpansive (projT1: @sigTO A P → leibnizO A).
+Proof. solve_proper. Qed.
+
+Lemma projT2_ne {A P}: ∀ n (x1 x2 : @sigTO A P) (Heq : x1 ≡{n}≡ x2),
+  rew (sigT_dist_proj1 n Heq) in projT2 x1 ≡{n}≡ projT2 x2.
+Proof. by destruct Heq. Qed.
+
+Section saved_ho_sem_type.
+  Context `{!savedHoSemTypeG vl Σ}.
+  Implicit Types (Ψ : packedFun vl Σ).
+
+  Definition packedFun_eq : packedFun vl Σ =
+    sigTO (λ n, vec n vl -d> (var → vl) -d> vl -d> laterO (iProp Σ)) := reflexivity _.
+
+  Definition packedFun_arity : packedFun vl Σ -n> natO := λne x, projT1 x.
+
+  Definition cpack n : hoEnvND n vl Σ → packedFun vl Σ :=
+    λ Φ, existT n (λ args ρ v, Next (Φ args ρ v)).
+
+  Global Instance cpack_contractive: Contractive (cpack n).
+  Proof.
+    rewrite /cpack => ?????.
+    apply (existT_ne _ eq_refl).
+    solve_contractive_ho.
+  Qed.
+
+  Program Definition pack : hoEnvDO vl Σ -n> packedFun vl Σ :=
+    λne Φ, cpack (projT1 Φ) (projT2 Φ).
+  Next Obligation.
+    move => n [i1 Φ1] [i2 Φ2][/= Heqi HeqΦ]. destruct Heqi. by f_equiv.
+  Qed.
+
+  Definition saved_ho_sem_type_own γ n (Φ : hoEnvND n vl Σ) : iProp Σ :=
+    saved_anything_own (F := hoEnvDOF vl) γ (pack (existT n Φ)).
+
+  Notation "γ ⤇[ n  ] φ" := (saved_ho_sem_type_own γ n φ) (at level 20).
+
+  Instance saved_ho_sem_type_own_contractive γ i : Contractive (saved_ho_sem_type_own γ i).
+  Proof.
+    rewrite /saved_ho_sem_type_own => n f g /= Heq. f_equiv.
+    apply (existT_ne _ eq_refl) => ??? /=.
+    solve_contractive_ho.
+  Qed.
+
+  Lemma saved_ho_sem_type_alloc i φ : (|==> ∃ γ, γ ⤇[ i ] φ)%I.
+  Proof. apply saved_anything_alloc. Qed.
+
+  Lemma packedFun_arity_neI Ψ1 Ψ2 : Ψ1 ≡ Ψ2 ⊢@{iPropI Σ}
+    packedFun_arity Ψ1 ≡ packedFun_arity Ψ2.
+  Proof. exact: f_equiv. Qed.
+
+  Lemma packedFun_arity_neI2 Ψ1 Ψ2 : Ψ1 ≡ Ψ2 ⊢@{iPropI Σ}
+    ⌜ packedFun_arity Ψ1 = packedFun_arity Ψ2 ⌝.
+  Proof. rewrite packedFun_arity_neI; auto. Qed.
+
+  Lemma saved_ho_sem_type_agree_arity γ {i j Φ1 Φ2}:
+    γ ⤇[ i ] Φ1 -∗ γ ⤇[ j ] Φ2 -∗ ⌜ i = j ⌝.
+  Proof.
+    iIntros "HΦ1 HΦ2 /=".
+    (* iDestruct (packedFun_arity_neI2 with "[HΦ1 HΦ2]") as "?".
+    iApply (saved_anything_agree with "HΦ1 HΦ2"). done. *)
+    (* Fail iDestruct (packedFun_arity_neI2 $! (saved_anything_agree with "HΦ1 HΦ2")) as "?". *)
+    iDestruct (saved_anything_agree with "HΦ1 HΦ2") as "Heq".
+    (* iDestruct (packedFun_arity_neI2 with "Heq") as "?". *)
+    rewrite packedFun_arity_neI2. done.
+  Qed.
+
+  Lemma saved_ho_sem_type_agree γ n (Φ1 Φ2 : hoEnvND n vl Σ) a b c:
+    γ ⤇[ n ] Φ1 -∗ γ ⤇[ n ] Φ2 -∗ ▷ (Φ1 a b c ≡ Φ2 a b c).
+  Proof.
+    iIntros "HΦ1 HΦ2 /=".
+    iDestruct (saved_anything_agree with "HΦ1 HΦ2") as "Heq".
+    rewrite /= sigT_equivI. iDestruct "Heq" as (Heq) "Heq".
+    rewrite (proof_irrel Heq eq_refl) /=.
+    repeat setoid_rewrite bi.discrete_fun_equivI; iNext.
+    iApply "Heq".
+  Qed.
+
+  Lemma saved_ho_sem_type_agree_dep γ {i j Φ1 Φ2} a b c:
+    γ ⤇[ i ] Φ1 -∗ γ ⤇[ j ] Φ2 -∗ ∃ eq : i = j,
+    ▷ ((rew [hoEnvD_P vl Σ] eq in Φ1) a b c ≡ Φ2 a b c).
+  Proof.
+    iIntros "HΦ1 HΦ2 /=".
+    iDestruct (saved_ho_sem_type_agree_arity with "HΦ1 HΦ2") as %->.
+    iExists eq_refl; cbn.
+    iApply (saved_ho_sem_type_agree with "HΦ1 HΦ2").
+  Qed.
+End saved_ho_sem_type.
+
+Notation "γ ⤇[ n  ] φ" := (saved_ho_sem_type_own γ n φ) (at level 20).
+Global Opaque saved_ho_sem_type_own.
